theories/Translations/LustreAstToLustre.v
@@ -23,17 +23,78 @@ Proof.
   all: discriminate.
 Qed.
 
-Record common_temp : Set := {
+From Stdlib Require FMaps.
+
+Module StringKey.
+  Definition t : Type := string.
+  Definition eq (s1 s2 : t) := s1 = s2.
+  Definition lt (s1 s2 : t) := ltb s1 s2 = true.
+  Definition eq_refl : forall s : t, eq s s := @eq_refl _.
+  Definition eq_sym : forall s1 s2 : t, eq s1 s2 -> eq s2 s1 := @eq_sym _.
+  Definition eq_trans : forall s1 s2 s3 : t, eq s1 s2 -> eq s2 s3 -> eq s1 s3 := @eq_trans _.
+  Definition lt_trans : forall s1 s2 s3 : t, lt s1 s2 -> lt s2 s3 -> lt s1 s3.
+  Proof using.
+    unfold lt, ltb.
+    intros s1 s2 s3 H12 H23.
+    induction s1 as [|c1 s1 IH1] in s2, s3, H12, H23 |- *.
+    1: destruct s2; [discriminate H12|destruct s3; [discriminate H23|reflexivity]].
+    destruct s2 as [|c2 s2]; [discriminate H12|].
+    destruct s3 as [|c3 s3]; [discriminate H23|].
+    cbn in *.
+    destruct (Ascii.compare c1 c2) as [| |] eqn:eq12; [apply Ascii.compare_eq_iff in eq12; subst c1|clear H12|discriminate H12].
+    1: destruct (Ascii.compare c2 c3); [exact (IH1 _ _ H12 H23)|reflexivity|discriminate H23].
+    destruct (Ascii.compare c2 c3) eqn:eq23; [| |discriminate H23].
+    1: apply Ascii.compare_eq_iff in eq23; subst c3; rewrite eq12; reflexivity.
+    unfold Ascii.compare in eq12; rewrite BinNat.N.compare_lt_iff in eq12.
+    unfold Ascii.compare in eq23; rewrite BinNat.N.compare_lt_iff in eq23.
+    specialize (BinNat.N.lt_trans _ _ _ eq12 eq23) as lt13.
+    apply BinNat.N.compare_lt_iff in lt13.
+    unfold Ascii.compare; rewrite lt13.
+    reflexivity.
+  Defined.
+  Definition lt_not_eq : forall s1 s2 : t, lt s1 s2 -> ~ eq s1 s2.
+  Proof using.
+    intros s ? H <-.
+    induction s as [|c s IH]; [discriminate H|refine (IH _)].
+    unfold lt, ltb, compare, Ascii.compare in *; fold compare in *.
+    rewrite (BinNat.N.compare_refl _) in H.
+    exact H.
+  Defined.
+  Definition compare : forall s1 s2 : t, OrderedType.Compare lt eq s1 s2.
+  Proof using.
+    intros s1 s2; destruct (String.compare s1 s2) eqn:eqcmp;
+      [refine (OrderedType.EQ _)|refine (OrderedType.LT _)|refine (OrderedType.GT _)].
+    1: apply String.compare_eq_iff; exact eqcmp.
+    1: unfold lt, ltb; rewrite eqcmp; reflexivity.
+    1: unfold lt, ltb; rewrite String.compare_antisym, eqcmp; reflexivity.
+  Defined.
+  Definition eq_dec : forall s1 s2 : t, { eq s1 s2 } + { ~ eq s1 s2 } := String.string_dec.
+End StringKey.
+Module StringMap <: FMapInterface.S with Module E := StringKey := FMapList.Make(StringKey).
+
+Record common_temp : Type := {
   orig :> Source.node;
-  env: Dict.t Target.type;
-  Henv: forall x t, Dict.maps_to x (convert_type t) env <-> In (x, t) (orig.(Source.n_in) ++ orig.(Source.n_out) ++ orig.(Source.n_locals));
   
+  smap: StringMap.t (ident * Result.declaration_location);
   n_in: list Target.binder;
   n_out: list Target.binder;
   n_locals: list Target.binder;
   
   nvars := n_in ++ n_out ++ n_locals;
-  Hnvars: nvars = map (fun '(x, t) => (x, convert_type t)) (orig.(Source.n_in) ++ orig.(Source.n_out) ++ orig.(Source.n_locals));
+  Hnvars:
+    Forall2 (fun '(x, tx) '(l, (v, tv)) =>
+        StringMap.find v smap = Some (x, l) /\
+        tx = convert_type tv)
+      nvars
+      (map (pair Result.DeclInput) orig.(Source.n_in) ++
+       map (pair Result.DeclOutput) orig.(Source.n_out) ++
+       map (pair Result.DeclLocal) orig.(Source.n_locals));
+  
+  seed: ident;
+  Hseed: forall n, ~ In (iter n next_ident seed) (map fst nvars);
+  
+  env: Dict.t Target.type;
+  Henv: forall x t, Dict.maps_to x t env <-> In (x, t) (n_in ++ n_out ++ n_locals);
 }.
 
 Definition translate_unop (op: Source.unop): { tin & { tout & Target.unop tin tout } } := match op with
@@ -76,16 +137,22 @@ Proof.
       exact (Target.EConst (Target.CBool b)).
     + exists Target.TInt.
       exact (Target.EConst (Target.CInt n)).
-  - destruct (Dict.find n (env temp)) as [ ty | ].
-    2: right; exact [(l, Result.UndeclaredInput n)].
+  - destruct (StringMap.find n (smap temp)) as [ [ i l' ] | ].
+    2: right; exact [(l, Result.UndeclaredInput n None)].
+    refine (match l' with Result.DeclInput => _ | _ => Result.Err [(l, Result.UndeclaredInput n (Some i))] end).
+    clear l'.
+    destruct (Dict.find i (env temp)) as [ ty | ].
+    2: right; exact [(l, Result.InternalError ("Input " ++ n ++ " has an ID but no type"))].
     left.
     exists ty.
-    exact (Target.EInput (n, ty)).
-  - destruct (Dict.find n (env temp)) as [ ty | ].
+    exact (Target.EInput (i, ty)).
+  - destruct (StringMap.find n (smap temp)) as [ [ i _ ] | ].
     2: right; exact [(l, Result.UndeclaredVariable n)].
+    destruct (Dict.find i (env temp)) as [ ty | ].
+    2: right; exact [(l, Result.InternalError ("Variable " ++ n ++ " has an ID but no type"))].
     left.
     exists ty.
-    exact (Target.EVar (n, ty)).
+    exact (Target.EVar (i, ty)).
   - refine (Result.bind (check_exp temp e) _).
     intros e'.
     destruct (translate_unop op) as [ tin [ tout top ]].
@@ -126,16 +193,18 @@ Proof.
     exact (incl_nil_l _).
   - refine (Result.bind (Result.combine (check_exp temp e) IH) _); clear IH.
     intros [ [ ty e' ] [ eqs IH ] ].
-    destruct (In_dec (prod_dec PeanoNat.Nat.eq_dec Target.type_dec) (n, ty) (nvars temp)) as [Hin|_].
+    destruct (StringMap.find n (smap temp)) as [ [ i l' ] | ].
+    2: exact (Result.Err [(l, Result.UndeclaredVariable n)]).
+    destruct (In_dec (prod_dec PeanoNat.Nat.eq_dec Target.type_dec) (i, ty) (nvars temp)) as [Hin|_].
     2: refine (Result.Err [(l, _)]).
-    2: destruct temp as [? ? ? ? ? ? nvars H]; cbn; fold nvars; clear H IH; generalize dependent nvars; intros nvars; clear - l n ty nvars.
+    2: destruct temp as [? ? ? ? ? nvars H ? H']; cbn; fold nvars; clear H H' IH; generalize dependent nvars; intros nvars; clear - n i ty nvars.
     2: induction nvars as [|[hdn hdt] tl IH].
-    2:  exact (Result.NeverAssigned n ty).
-    2: destruct (PeanoNat.Nat.eq_dec n hdn) as [neqhdn|_].
+    2:  exact (Result.UndeclaredVariable n).
+    2: destruct (PeanoNat.Nat.eq_dec i hdn) as [neqhdn|_].
     2:  exact (Result.IncompatibleTypeAssignment hdn hdt ty).
     2: exact IH.
     left.
-    exists ((n, existT Target.exp ty e') :: eqs).
+    exists ((i, existT Target.exp ty e') :: eqs).
     intros a [<-|H]; [exact Hin|exact (IH _ H)].
 Defined.
 
@@ -144,39 +213,19 @@ Definition n_assigned_vars (body: list Target.equation) :=
 
 Scheme Equality for list.
 
-Module EquationOrder <: Orders.TotalLeBool.
-  Local Coercion is_true : bool >-> Sortclass.
-
-  Definition t := Source.equation.
-
-  Definition leb (x y: Source.equation): bool := Nat.leb (fst x) (fst y).
-  Infix "<=?" := leb (at level 70, no associativity).
-
-  Theorem leb_total: forall x y, x <=? y \/ y <=? x.
-  Proof.
-    intros [] [].
-    unfold leb; simpl.
-
-    revert i i0.
-    induction i; destruct i0; simpl; auto.
-  Qed.
-End EquationOrder.
-
-Module Import EquationSort := Sort EquationOrder.
-
 Definition check_assigned_out (l: Result.location) (temp: common_temp) body: Result.t Target.type (incl (n_out temp) (n_assigned_vars body)).
 Proof.
   refine (Result.bind (Result.list_map _ _) (fun H => Result.Ok (proj2 (incl_Forall_in_iff _ _) H))).
   intros b.
   destruct (In_dec (prod_dec PeanoNat.Nat.eq_dec Target.type_dec) b (n_assigned_vars body)) as [Hin|Hnin].
   1: exact (Result.Ok Hin).
-  exact (Result.Err [(l, Result.NeverAssigned (fst b) (snd b))]).
+  exact (Result.Err [(l, Result.NeverAssigned "<information lost>" (fst b) (snd b))]).
 Defined.
 
 Definition n_out_is_not_an_input (l: Result.location) (temp: common_temp) :
   Result.t Target.type (Forall (fun b => ~ In (fst b) (map fst (n_in temp))) (n_out temp)) :=
   Result.list_map (fun b => match In_dec PeanoNat.Nat.eq_dec _ _ with
-    | left _ => Result.Err [(l, Result.MultipleDeclaration (fst b) Result.DeclInput Result.DeclOutput)]
+    | left _ => Result.Err [(l, Result.MultipleDeclaration "<information lost>" (fst b) Result.DeclInput Result.DeclOutput)]
     | right h => Result.Ok h
   end) _.
 
@@ -211,51 +260,161 @@ Proof using.
   left; intros []; assumption.
 Defined.
 
-Import Result.notations.
-
-Lemma check_Henv {entry} :
-  let n_in := map (fun '(n, t) => (n, convert_type t)) (Source.n_in entry) in
-  let n_out := map (fun '(n, t) => (n, convert_type t)) (Source.n_out entry) in
-  let n_locals := map (fun '(n, t) => (n, convert_type t)) (Source.n_locals entry) in
-  Result.t Target.type (forall n t,
-    Dict.maps_to n (convert_type t)
-      (fold_left (fun acc '(n, t) => Dict.add n t acc)
-      (n_in ++ n_out ++ n_locals)
-      (Dict.empty Target.type)) <->
-    In (n, t) (Source.n_in entry ++ Source.n_out entry ++ Source.n_locals entry)).
+Lemma Forall_univ : forall [A] (P : A -> Prop), (forall x, P x) -> forall l, Forall P l.
 Proof using.
-  destruct entry as [l ? nin nout nloc ?]; cbn; clear - l.
-  refine (Result.bind
-    (Result.combine_prop (Result.list_map (P := fun v => forall ty', In (fst v, ty') nin -> ty' = snd v) _ nin)
-    (Result.combine_prop (Result.list_map (P := fun v => ~ In (fst v) (map fst nout)) _ nin)
-    (Result.combine_prop (Result.list_map (P := fun v => ~ In (fst v) (map fst nloc)) _ nin)
-    (Result.combine_prop (Result.list_map (P := fun v => forall ty', In (fst v, ty') nout -> ty' = snd v) _ nout)
-    (Result.combine_prop (Result.list_map (P := fun v => ~ In (fst v) (map fst nloc)) _ nout)
-                         (Result.list_map (P := fun v => forall ty', In (fst v, ty') nloc -> ty' = snd v) _ nloc)))))) _).
-  all: try refine (fun v => match In_dec PeanoNat.Nat.eq_dec _ _ with left _ => _ | right h => Result.Ok h end).
-  1: rename nin into nlist.
-  4: rename nout into nlist.
-  6: rename nloc into nlist.
-  1-6: try (intros [b t]; refine (match forall_type_dec (* Technically, does not check for duplicates, only variables with same ID but different types *)
-        (fun ty' => In (b, ty') nlist -> ty' = t)
-        ltac:(
-          intros ty;
-          destruct (In_dec (prod_dec PeanoNat.Nat.eq_dec Source.type_dec) (b, ty) nlist) as [Hin|Hnin]; [|left; intros f; contradiction (Hnin f)];
-          destruct (Source.type_dec ty t) as [eqty|nety]; [left; intros _; exact eqty|];
-          right; intros f; exact (nety (f Hin)))
-        with left h => Result.Ok h | right _ => _ end)).
-  1: exact (Result.Err [(l, Result.MultipleDeclaration b Result.DeclInput Result.DeclInput)]).
-  1: exact (Result.Err [(l, Result.MultipleDeclaration (fst v) Result.DeclInput Result.DeclOutput)]).
-  1: exact (Result.Err [(l, Result.MultipleDeclaration (fst v) Result.DeclInput Result.DeclLocal)]).
-  1: exact (Result.Err [(l, Result.MultipleDeclaration b Result.DeclOutput Result.DeclOutput)]).
-  1: exact (Result.Err [(l, Result.MultipleDeclaration (fst v) Result.DeclOutput Result.DeclLocal)]).
-  1: exact (Result.Err [(l, Result.MultipleDeclaration b Result.DeclLocal Result.DeclLocal)]).
-  intros (innotdup' & innotout' & innotloc' & outnotdup' & outnotloc' & locnotdup').
-  left; intros n t.
+  intros A P HP l; induction l as [|hd tl IH]; constructor; [exact (HP _)|exact IH].
+Qed.
+
+Definition build_map (entry: Source.node) :
+  { sm & { seed & Result.t Target.type { n_in & { n_out & { n_locals |
+    Forall (fun v => forall ty', In (fst v, ty') n_in -> ty' = snd v) n_in /\
+    Forall (fun v => forall ty', In (fst v, ty') n_out -> ty' = snd v) n_out /\
+    Forall (fun v => forall ty', In (fst v, ty') n_locals -> ty' = snd v) n_locals /\
+    Forall (fun v => ~ In (fst v) (map fst n_out)) n_in /\
+    Forall (fun v => ~ In (fst v) (map fst n_locals)) n_in /\
+    Forall (fun v => ~ In (fst v) (map fst n_locals)) n_out /\
+    Forall2 (fun '(x, tx) '(l, (v, tv)) =>
+        StringMap.find v sm = Some (x, l) /\
+        tx = convert_type tv)
+      (n_in ++ n_out ++ n_locals)
+      (map (pair Result.DeclInput) entry.(Source.n_in) ++
+       map (pair Result.DeclOutput) entry.(Source.n_out) ++
+       map (pair Result.DeclLocal) entry.(Source.n_locals)) /\
+    (forall n, ~ In (iter n next_ident seed) (map fst (n_in ++ n_out ++ n_locals))) } } } } }.
+Proof using.
+  destruct entry as [l n nin out loc body]; unfold Source.n_in, Source.n_out, Source.n_locals; clear n body.
+  induction nin as [ | [n ty] vars (sm & seed & IH) ].
+  2:{
+    destruct (StringMap.find n sm) as [ [ i dl ] | ] eqn:eqnsm.
+    1: exists sm, seed;
+       refine (Result.Err ((l, Result.MultipleDeclaration n i Result.DeclInput dl) :: match IH with Result.Ok _ => [] | Result.Err es => es end)).
+    exists (StringMap.add n (seed, Result.DeclInput) sm), (next_ident seed);
+      refine (Result.bind IH _);
+      intros (IHnin & IHout & IHloc & IHii & IHoo & IHll & IHio & IHil & IHol & IH1 & IH2);
+      left; exists ((seed, convert_type ty) :: IHnin), IHout, IHloc; repeat split; try assumption.
+    + constructor; [intros ty' [[=<-]|H]; [exact eq_refl|exfalso; refine (IH2 O _)]|].
+      1: rewrite map_app; exact (in_or_app _ _ _ (or_introl (in_map fst _ _ H))).
+      assert (Hseed : ~ In seed (map fst IHnin))
+        by (rewrite map_app in IH2; exact (fun f => IH2 O (in_or_app _ _ _ (or_introl f)))).
+      clear - IHii Hseed.
+      refine (proj2 (Forall_forall _ _) _).
+      intros [v tv] Hv ty' [[=f _]|H]; [contradict Hseed; subst; exact (in_map fst _ _ Hv)|].
+      exact (proj1 (Forall_forall _ _) IHii _ Hv _ H).
+    + constructor; [|assumption]. refine (fun f => IH2 O _).
+      rewrite map_app; refine (in_or_app _ _ _ (or_intror _)).
+      rewrite map_app; exact (in_or_app _ _ _ (or_introl f)).
+    + constructor; [|assumption]. refine (fun f => IH2 O _).
+      rewrite map_app; refine (in_or_app _ _ _ (or_intror _)).
+      rewrite map_app; exact (in_or_app _ _ _ (or_intror f)).
+    + constructor; [split; [|exact eq_refl]|].
+      1: exact (StringMap.find_1 (StringMap.add_1 _ _ eq_refl)).
+      refine (Forall2_impl _ _ IH1); clear - eqnsm.
+      intros [x tx] [l' [v tv]] [H1 H2]; split; [clear tx tv H2|exact H2].
+      refine (StringMap.find_1 (StringMap.add_2 _ _ (StringMap.find_2 H1))).
+      intros <-; rewrite eqnsm in H1; discriminate H1.
+    + intros k [H|H]; [|exact (eq_ind _ (fun v => ~ In v _) (IH2 (S k)) _ (PeanoNat.Nat.iter_succ_r _ _ _ _) H)].
+      cbn in H; clear - H.
+      assert (tmp : seed < iter k next_ident (S seed)); [|rewrite H in tmp at 1; exact (PeanoNat.Nat.lt_irrefl _ tmp)].
+      induction k as [|n IH] in seed |- *; [exact (le_n _)|].
+      exact (le_S _ _ (IH _)).
+  }
+  refine (match _ : { sm & { seed & Result.t _ { n_out & { n_locals |
+                      _ /\ _ /\ _ /\ Forall2 _ (n_out ++ _) (map _ out ++ _) /\ (forall n, ~ In _ (map _ (n_out ++ _)))}}}} with
+    | existT _ sm (existT _ seed (Result.Ok (existT _ n_out (exist _ n_locals (conj Hoo (conj Hll (conj Hol (conj H1 H2)))))))) =>
+        existT _ sm (existT _ seed (Result.Ok (
+          existT _ [] (existT _ n_out (exist _ n_locals
+            (conj (Forall_nil _) (conj Hoo (conj Hll (conj (Forall_nil _) (conj (Forall_nil _) (conj Hol (conj H1 H2))))))))))))
+    | existT _ sm (existT _ seed (Result.Err e)) => existT _ sm (existT _ seed (Result.Err e)) end).
+  induction out as [ | [n ty] vars (sm & seed & IH) ].
+  2:{
+    destruct (StringMap.find n sm) as [ [ i dl ] | ] eqn:eqnsm.
+    1: exists sm, seed;
+       refine (Result.Err ((l, Result.MultipleDeclaration n i Result.DeclOutput dl) :: match IH with Result.Ok _ => [] | Result.Err es => es end)).
+    exists (StringMap.add n (seed, Result.DeclOutput) sm), (next_ident seed);
+      refine (Result.bind IH _);
+      intros (IHout & IHloc & IHoo & IHll & IHol & IH1 & IH2);
+      left; exists ((seed, convert_type ty) :: IHout), IHloc; repeat split; try assumption.
+    + constructor; [intros ty' [[=<-]|H]; [exact eq_refl|exfalso; refine (IH2 O _)]|].
+      1: rewrite map_app; exact (in_or_app _ _ _ (or_introl (in_map fst _ _ H))).
+      assert (Hseed : ~ In seed (map fst IHout))
+        by (rewrite map_app in IH2; exact (fun f => IH2 O (in_or_app _ _ _ (or_introl f)))).
+      clear - IHoo Hseed.
+      refine (proj2 (Forall_forall _ _) _).
+      intros [v tv] Hv ty' [[=f _]|H]; [contradict Hseed; subst; exact (in_map fst _ _ Hv)|].
+      exact (proj1 (Forall_forall _ _) IHoo _ Hv _ H).
+    + constructor; [|assumption]. refine (fun f => IH2 O _).
+      rewrite map_app; exact (in_or_app _ _ _ (or_intror f)).
+    + constructor; [split; [|exact eq_refl]|].
+      1: exact (StringMap.find_1 (StringMap.add_1 _ _ eq_refl)).
+      refine (Forall2_impl _ _ IH1); clear - eqnsm.
+      intros [x tx] [l' [v tv]] [H1 H2]; split; [clear tx tv H2|exact H2].
+      refine (StringMap.find_1 (StringMap.add_2 _ _ (StringMap.find_2 H1))).
+      intros <-; rewrite eqnsm in H1; discriminate H1.
+    + intros k [H|H]; [|exact (eq_ind _ (fun v => ~ In v _) (IH2 (S k)) _ (PeanoNat.Nat.iter_succ_r _ _ _ _) H)].
+      cbn in H; clear - H.
+      assert (tmp : seed < iter k next_ident (S seed)); [|rewrite H in tmp at 1; exact (PeanoNat.Nat.lt_irrefl _ tmp)].
+      induction k as [|n IH] in seed |- *; [exact (le_n _)|].
+      exact (le_S _ _ (IH _)).
+  }
+  refine (match _ : { sm & { seed & Result.t _ { n_locals |
+                      _ /\ Forall2 _ n_locals (map _ _) /\ (forall n, ~ In _ (map _ n_locals))}}} with
+    | existT _ sm (existT _ seed (Result.Ok (exist _ n_locals (conj Hll (conj H1 H2))))) =>
+        existT _ sm (existT _ seed (Result.Ok (
+          existT _ [] (exist _ n_locals
+            (conj (Forall_nil _) (conj Hll (conj (Forall_nil _) (conj H1 H2))))))))
+    | existT _ sm (existT _ seed (Result.Err e)) => existT _ sm (existT _ seed (Result.Err e)) end).
+  induction loc as [ | [n ty] vars (sm & seed & IH) ].
+  2:{
+    destruct (StringMap.find n sm) as [ [ i dl ] | ] eqn:eqnsm.
+    1: exists sm, seed;
+       refine (Result.Err ((l, Result.MultipleDeclaration n i Result.DeclLocal dl) :: match IH with Result.Ok _ => [] | Result.Err es => es end)).
+    exists (StringMap.add n (seed, Result.DeclLocal) sm), (next_ident seed);
+      refine (Result.bind IH _);
+      intros (IHloc & IHll & IH1 & IH2);
+      left; exists ((seed, convert_type ty) :: IHloc); repeat split; try assumption.
+    + constructor; [intros ty' [[=<-]|H]; [exact eq_refl|exfalso; refine (IH2 O _)]|].
+      1: exact (in_map fst _ _ H).
+      assert (Hseed : ~ In seed (map fst IHloc))
+        by (exact (fun f => IH2 O f)).
+      clear - IHll Hseed.
+      refine (proj2 (Forall_forall _ _) _).
+      intros [v tv] Hv ty' [[=f _]|H]; [contradict Hseed; subst; exact (in_map fst _ _ Hv)|].
+      exact (proj1 (Forall_forall _ _) IHll _ Hv _ H).
+    + constructor; [split; [|exact eq_refl]|].
+      1: exact (StringMap.find_1 (StringMap.add_1 _ _ eq_refl)).
+      refine (Forall2_impl _ _ IH1); clear - eqnsm.
+      intros [x tx] [l' [v tv]] [H1 H2]; split; [clear tx tv H2|exact H2].
+      refine (StringMap.find_1 (StringMap.add_2 _ _ (StringMap.find_2 H1))).
+      intros <-; rewrite eqnsm in H1; discriminate H1.
+    + intros k [H|H]; [|exact (eq_ind _ (fun v => ~ In v _) (IH2 (S k)) _ (PeanoNat.Nat.iter_succ_r _ _ _ _) H)].
+      cbn in H; clear - H.
+      assert (tmp : seed < iter k next_ident (S seed)); [|rewrite H in tmp at 1; exact (PeanoNat.Nat.lt_irrefl _ tmp)].
+      induction k as [|n IH] in seed |- *; [exact (le_n _)|].
+      exact (le_S _ _ (IH _)).
+  }
+  exists (StringMap.empty _), O; left; exists []; split; [exact (Forall_nil _)|split; [exact (Forall2_nil _)|intros ? f; exact f]].
+Defined.
+
+Lemma check_Henv {n_in n_out n_loc} :
+  Forall (fun v => forall ty', In (fst v, ty') n_in -> ty' = snd v) n_in ->
+  Forall (fun v => forall ty', In (fst v, ty') n_out -> ty' = snd v) n_out ->
+  Forall (fun v => forall ty', In (fst v, ty') n_loc -> ty' = snd v) n_loc ->
+  Forall (fun v => ~ In (fst v) (map fst n_out)) n_in ->
+  Forall (fun v => ~ In (fst v) (map fst n_loc)) n_in ->
+  Forall (fun v => ~ In (fst v) (map fst n_loc)) n_out ->
+  forall n t,
+    Dict.maps_to n t
+      (fold_left (fun acc '(n, t) => Dict.add n t acc)
+       (n_in ++ n_out ++ n_loc)
+       (Dict.empty Target.type)) <->
+    In (n, t) (n_in ++ n_out ++ n_loc)%list.
+Proof using.
+  rename n_in into nin, n_out into nout, n_loc into nloc.
+  intros innotdup' outnotdup' locnotdup' innotout' innotloc' outnotloc' n t.
   match goal with |- Dict.maps_to _ _ (fold_left ?f ?l ?d) <-> _ =>
   rewrite <-(fold_left_rev_right (fun x y => f y x) l d) end.
   rewrite (in_rev (nin ++ nout ++ nloc) (n, t)),
-          !rev_app_distr, <-!app_assoc, <-!map_rev.
+          !rev_app_distr, <-!app_assoc.
   apply Forall_rev in innotdup', innotloc', innotout', outnotloc', outnotdup', locnotdup'.
   specialize (Forall_impl _ (fun v HP ty' Hin => HP ty' (proj2 (in_rev _ _) Hin)) innotdup') as innotdup.
   specialize (Forall_impl _ (fun v Hnin Hin => Hnin (proj2 (in_rev _ _) (eq_ind _ _ Hin _ (map_rev _ _)))) innotout') as innotout.
@@ -266,7 +425,7 @@ Proof using.
   remember (rev nin) as l3 eqn:eq3.
   remember (rev nout) as l2 eqn:eq2.
   remember (rev nloc) as l1 eqn:eq1.
-  clear l nin nout nloc eq1 eq2 eq3 innotdup' innotout' innotloc' outnotdup' outnotloc' locnotdup'.
+  clear nin nout nloc eq1 eq2 eq3 innotdup' innotout' innotloc' outnotdup' outnotloc' locnotdup'.
   split.
   - intros H.
     clear innotout innotloc outnotloc.
@@ -329,21 +488,26 @@ Proof using.
     1-3: clear; intros x H t Hin; exact (H _ (or_intror Hin)).
 Defined.
 
+Import Result.notations.
+
 Definition check_node_prop (entry: Source.node): Result.t Target.type Target.node :=
-  let n_in := map (fun '(n, t) => (n, convert_type t)) (Source.n_in entry) in
-  let n_out := map (fun '(n, t) => (n, convert_type t)) (Source.n_out entry) in
-  let n_locals := map (fun '(n, t) => (n, convert_type t)) (Source.n_locals entry) in
-  do Henv <- check_Henv;
+  let '(existT _ sm (existT _ seed tmp)) := build_map entry in
+  do '(existT _ n_in (existT _ n_out (exist _ n_loc
+        (conj Hii (conj Hoo (conj Hll (conj Hio (conj Hil (conj Hol (conj Hnvars Hseed)))))))))) <- tmp;
+  let Henv := check_Henv Hii Hoo Hll Hio Hil Hol in
   let temp := {|
     orig := entry;
-    env := fold_left (fun acc '(n, t) => Dict.add n t acc) (n_in ++ n_out ++ n_locals) (Dict.empty _);
-    Henv := Henv;
-    
     n_in := n_in;
     n_out := n_out;
-    n_locals := n_locals;
+    n_locals := n_loc;
     
-    Hnvars := eq_sym (eq_trans (map_app _ _ _) (f_equal _ (map_app _ _ _)));
+    Hnvars := Hnvars;
+    
+    seed := seed;
+    Hseed := Hseed;
+    
+    env := fold_left (fun acc '(n, t) => Dict.add n t acc) (n_in ++ n_out ++ n_loc) (Dict.empty _);
+    Henv := Henv;
   |} in
   do '(exist _ n_body assigned_vars_are_vars) <- check_body temp entry;
   do '(conj check_assigned (conj n_out_is_not_an_input (conj n_inputs_equations n_no_einputs_in_other))) <-
@@ -356,11 +520,13 @@ Definition check_node_prop (entry: Source.node): Result.t Target.type Target.nod
       Target.n_name := Source.n_name entry;
       Target.n_in := n_in;
       Target.n_out := n_out;
-      Target.n_locals := n_locals;
+      Target.n_locals := n_loc;
       Target.n_body := n_body;
       Target.n_assigned_vars_are_vars := assigned_vars_are_vars;
       Target.n_assigned_out := check_assigned;
       Target.n_out_is_not_an_input := n_out_is_not_an_input;
       Target.n_inputs_equations := n_inputs_equations;
-      Target.n_no_einputs_in_other := n_no_einputs_in_other
+      Target.n_no_einputs_in_other := n_no_einputs_in_other;
+      Target.n_seed := seed;
+      Target.n_seed_always_fresh := Hseed;
     |}.
