extracted/Extractor.v
@@ -5,7 +5,7 @@ From Stdlib Require Import ExtrOcamlBasic ExtrOcamlNatInt ExtrOcamlNativeString.
 
 #[local] Set Warnings "-extraction-default-directory".
 
-
+Extract Constant String.compare => "StringImpl.compare".
 Extract Constant LustreOrdering.node_ordering => "Ordered.node_ordering".
 Extract Constant Base.ABORT_FIXME => "Abort.aBORT_FIXME".
 
