theories/Languages/LustreAst.v
@@ -10,7 +10,7 @@ Inductive type: Type :=
   | TBool
   | TInt.
 
-Definition binder := ident.
+Definition binder := string.
 
 Inductive const: Type :=
   | CVoid: const
@@ -80,7 +80,7 @@ Fixpoint has_einput (e: exp): bool :=
     | EIfte _ e1 e2 e3 => has_einput e1 || has_einput e2 || has_einput e3
   end.
 
-Definition equation: Set := ident * exp.
+Definition equation: Set := string * exp.
 
 
 Record node := mk_node {
@@ -101,22 +101,6 @@ Definition node_eq (n1 n2: node) :=
   Permutation (n_body n1) (n_body n2).
 
 Definition name_dec := String.string_dec.
-
-
-Fixpoint var_of_exp_aux (e: exp) (acc: list ident): list ident :=
-  match e with
-    | EConst _ _ => acc
-    | EInput _ _ => acc
-    | EVar _ name => name :: acc
-    | EUnop _ _ e => var_of_exp_aux e acc
-    | EBinop _ _ e1 e2 =>
-      var_of_exp_aux e1 (var_of_exp_aux e2 acc)
-    | EIfte _ e1 e2 e3 =>
-      var_of_exp_aux e1 (var_of_exp_aux e2 (var_of_exp_aux e3 acc))
-  end.
-
-Definition var_of_exp (e: exp): list ident :=
-  var_of_exp_aux e [].
 
 
 (** ** Equality of binders *)
@@ -150,38 +134,38 @@ Proof.
   all: right; inversion 1.
 Defined.
 
-Definition binder_eqb (x y: binder): bool := (x =? y).
+Definition binder_eqb (x y: binder): bool := (x =? y)%string.
 
 Lemma binder_eqb_eq (x y: binder):
   binder_eqb x y = true <-> x = y.
 Proof.
-  apply PeanoNat.Nat.eqb_eq.
+  apply String.eqb_eq.
 Qed.
 
 Lemma binder_dec (x y: binder): {x = y} + {x <> y}.
 Proof.
-  exact (PeanoNat.Nat.eq_dec x y).
+  exact (string_dec x y).
 Defined.
 
 Lemma binder_eqb_refl (b: binder):
   binder_eqb b b = true.
 Proof.
-  apply PeanoNat.Nat.eqb_refl.
+  apply String.eqb_refl.
 Qed.
 
 Lemma binder_eqb_to_eq (x y : binder): binder_eqb x y = true -> x = y.
 Proof.
   unfold binder_eqb, andb.
-  destruct (x =? y) eqn:Heq; [| discriminate ].
+  destruct (x =? y)%string eqn:Heq; [| discriminate ].
 
-  now rewrite PeanoNat.Nat.eqb_eq in Heq.
+  now rewrite String.eqb_eq in Heq.
 Qed.
 
 Lemma binder_eq_to_eqb (x y : binder): x = y -> binder_eqb x y = true.
 Proof.
   unfold binder_eqb.
   intros ->.
-  apply PeanoNat.Nat.eqb_refl.
+  apply String.eqb_refl.
 Qed.
 
 
@@ -486,7 +470,7 @@ Proof.
 Qed.
 
 Definition equation_eqb (eq1 eq2: equation): bool :=
-  (fst eq1 =? fst eq2) && (exp_eqb (snd eq1) (snd eq2)).
+  (fst eq1 =? fst eq2)%string && (exp_eqb (snd eq1) (snd eq2)).
 
 Definition equation_eq : equation -> equation -> Prop := fun eq1 eq2 => (fst eq1 = fst eq2) /\ (exp_eq (snd eq1) (snd eq2)).
 
@@ -494,7 +478,7 @@ Lemma equation_dec (e1 e2: equation) : { equation_eq e1 e2 } + { ~ equation_eq e
 Proof.
   destruct e1 as [ e1_name e1_exp ].
   destruct e2 as [ e2_name e2_exp ].
-  pose proof (PeanoNat.Nat.eq_dec e1_name e2_name) as H.
+  pose proof (string_dec e1_name e2_name) as H.
   destruct H.
   2: {
     right.
@@ -520,7 +504,7 @@ Proof.
   destruct eq as (i, e).
   apply andb_true_intro.
   split.
-  - apply PeanoNat.Nat.eqb_refl.
+  - apply String.eqb_refl.
   - apply exp_eqb_refl.
 Qed.
 
@@ -531,7 +515,7 @@ Proof.
   - intro H.
     destruct eq1, eq2.
     apply andb_prop in H as [ H1 H2 ].
-    apply PeanoNat.Nat.eqb_eq in H1.
+    apply String.eqb_eq in H1.
     apply exp_eqb_eq in H2.
     simpl in H1, H2.
     rewrite H1.
@@ -540,7 +524,7 @@ Proof.
     intros [eq H]; cbn in eq, H; subst i'.
     apply andb_true_intro.
     split.
-    1: exact (PeanoNat.Nat.eqb_refl _).
+    1: exact (String.eqb_refl _).
     apply exp_eqb_eq in H.
     exact H.
 Qed.
